specialized Wf to type

PPlusProperties.v
@@ -489,7 +489,7 @@ Section PPlusTraceInclusion.
       apply (WeakInclusions_flat_PermutationEquivLists_r _ _ H1 H2 H3 H4).
   Qed.
 
-  Theorem PPlusTraceInclusion_TraceInclusion (m m' : BaseModule) (Wfm : forall ty, WfMod ty (Base m)) (Wfm' : forall ty, WfMod ty (Base m')):
+  Theorem PPlusTraceInclusion_TraceInclusion (m m' : BaseModule) (Wfm: WfMod (Base m)) (Wfm': WfMod (Base m')):
     PPlusTraceInclusion m m' ->
     TraceInclusion (Base m) (Base m').
   Proof.
@@ -1930,16 +1930,16 @@ Proof.
     apply PPlusSubsteps_inlined_undef_Rule; auto.
 Qed.      
 
-Lemma WfActionT_inline_Rule ty (k : Kind) m (a : ActionT ty k) rn f:
+Lemma WfActionT_inline_Rule (k : Kind) m (a : ActionT type k) rn f:
   WfActionT m a ->
   WfActionT (inlineSingle_Rule_BaseModule f rn m) a.
 Proof.
   intros; induction H; econstructor; auto.
 Qed.
 
-Lemma WfActionT_inline_Rule_inline_action ty (k : Kind) m (a : ActionT ty k) rn (f : DefMethT):
+Lemma WfActionT_inline_Rule_inline_action (k : Kind) m (a : ActionT type k) rn (f : DefMethT):
   WfActionT m a ->
-  (forall v, WfActionT m (projT2 (snd f) ty v)) ->
+  (forall v, WfActionT m (projT2 (snd f) type v)) ->
   WfActionT (inlineSingle_Rule_BaseModule f rn m) (inlineSingle f a).
 Proof.
   induction 1; try econstructor; eauto.
@@ -1980,15 +1980,15 @@ Proof.
   simpl; destruct string_dec, a; simpl;rewrite IHl; reflexivity.
 Qed.
 
-Lemma WfMod_Rule_inlined ty m f rn :
-  WfMod ty (Base m) ->
+Lemma WfMod_Rule_inlined m f rn :
+  WfMod (Base m) ->
   In f (getMethods m) ->
-  WfMod ty (Base (inlineSingle_Rule_BaseModule f rn m)).
+  WfMod (Base (inlineSingle_Rule_BaseModule f rn m)).
 Proof.
   intros; inv H; econstructor; eauto.
   - inv HWfBaseModule.
     split; intros; simpl in *; dest; try inv HWfBaseModule; eauto; repeat split; intros; pose proof (H1 _ H0); auto.
-    + destruct (inlineSingle_Rule_BaseModule_dec ty _ _ _ _ H2).
+    + destruct (inlineSingle_Rule_BaseModule_dec type _ _ _ _ H2).
       * specialize (H _ H7); apply WfActionT_inline_Rule; auto.
       * dest.
         specialize (H _ H7).
@@ -2000,7 +2000,7 @@ Qed.
 
 Lemma PPlusStrongTraceInclusion_inlining_Rules_r m f rn :
   In f (getMethods m) ->
-  (forall ty, WfMod ty (Base m)) ->
+  (WfMod (Base m)) ->
   StrongPPlusTraceInclusion m (inlineSingle_Rule_BaseModule f rn m).
 Proof.
   unfold StrongPPlusTraceInclusion; induction 3; subst.
@@ -2009,7 +2009,7 @@ Proof.
     + constructor.
   - dest.
     pose proof H0 as sth.
-    specialize (H0 (fun _ => unit)).
+    specialize (H0).
       destruct (in_dec (RuleOrMeth_dec) (Rle rn) execs),(in_dec string_dec rn (map fst (getRules m))); inv H0.
     * rewrite in_map_iff in i0; dest; destruct x0; simpl in *; subst.
       destruct HWfBaseModule as [? [? [NoDupMeths [NoDupRegisters NoDupRle]]]].
@@ -2044,13 +2044,13 @@ Qed.
 
 Theorem TraceInclusion_inlining_Rules_r m f rn :
   In f (getMethods m) ->
-  (forall ty, WfMod ty (Base m)) ->
+  (WfMod (Base m)) ->
   TraceInclusion (Base m) (Base (inlineSingle_Rule_BaseModule f rn m)).
 Proof.
   intros.
   apply PPlusTraceInclusion_TraceInclusion; auto.
   intros.
-  specialize (H0 ty).
+  specialize (H0).
   apply (WfMod_Rule_inlined); auto.
   eauto using StrongPPlusTraceInclusion_PPlusTraceInclusion, PPlusStrongTraceInclusion_inlining_Rules_r.
 Qed.
@@ -2704,16 +2704,16 @@ Proof.
   specialize (H1 _ HInDef); assumption.
 Qed.
 
-Lemma WfActionT_inline_Meth ty (k : Kind) m (a : ActionT ty k) rn f:
+Lemma WfActionT_inline_Meth (k : Kind) m (a : ActionT type k) rn f:
   WfActionT m a ->
   WfActionT (inlineSingle_Meth_BaseModule f rn m) a.
 Proof.
   intros; induction H; econstructor; auto.
 Qed.
 
-Lemma WfActionT_inline_Meth_inline_action ty (k : Kind) m (a : ActionT ty k) gn (f : DefMethT):
+Lemma WfActionT_inline_Meth_inline_action (k : Kind) m (a : ActionT type k) gn (f : DefMethT):
   WfActionT m a ->
-  (forall v, WfActionT m (projT2 (snd f) ty v)) ->
+  (forall v, WfActionT m (projT2 (snd f) type v)) ->
   WfActionT (inlineSingle_Meth_BaseModule f gn m) (inlineSingle f a).
 Proof.
   induction 1; try econstructor; eauto.
@@ -2746,13 +2746,13 @@ Proof.
 Qed.
 
 Lemma WfMod_Meth_inlined m f gn :
-  (forall ty, WfMod ty (Base m)) ->
+  (WfMod (Base m)) ->
   In f (getMethods m) ->
-  (forall ty, WfMod ty (Base (inlineSingle_Meth_BaseModule f gn m))).
+  (WfMod (Base (inlineSingle_Meth_BaseModule f gn m))).
 Proof.
   intros.
   pose proof H as sth.
-  specialize (H ty).
+  specialize (H).
   inv H; econstructor; eauto.
   - split; intros; simpl in *; inv HWfBaseModule.
     + apply WfActionT_inline_Meth; auto.
@@ -2771,7 +2771,7 @@ Qed.
 
 Lemma PPlusStrongTraceInclusion_inlining_Meth_r m f gn :
   In f (getMethods m) ->
-  (forall ty, WfMod ty (Base m)) ->
+  (WfMod (Base m)) ->
   StrongPPlusTraceInclusion m (inlineSingle_Meth_BaseModule f gn m).
 Proof.
   unfold StrongPPlusTraceInclusion; induction 3; subst.
@@ -2785,7 +2785,7 @@ Proof.
       * constructor; auto; unfold WeakInclusion_flat; split; intro; auto.
     + destruct (in_dec string_dec gn (map fst (getMethods m))).
       * rewrite in_map_iff in i; dest.
-        specialize (H0 (fun _ => unit)).
+        specialize (H0).
         inv H0; destruct x0; simpl in *.
         destruct HWfBaseModule as [? [? [NoDupMeths [NoDupRegisters NoDupRle]]]].
         specialize (PPlusStep_inline_Meth_In _ _ H5 H NoDupRle NoDupMeths n HPPlusStep) as TMP; dest.
@@ -2805,7 +2805,7 @@ Qed.
 
 Theorem TraceInclusion_inlining_Meth_r m f gn :
   In f (getMethods m) ->
-  (forall ty, WfMod ty (Base m)) ->
+  (WfMod (Base m)) ->
   TraceInclusion (Base m) (Base (inlineSingle_Meth_BaseModule f gn m)).
 Proof.
   intros.
@@ -2993,15 +2993,15 @@ Qed.
 
 Lemma WfMod_inline_all_Meth regs rules meths f xs:
   In f meths ->
-  (forall ty, WfMod ty (Base (BaseMod regs rules meths))) ->
-  (forall ty, WfMod ty (Base (BaseMod regs rules (fold_right (transform_nth_right (inlineSingle_Meth f)) meths xs)))).
+  (WfMod (Base (BaseMod regs rules meths))) ->
+  (WfMod (Base (BaseMod regs rules (fold_right (transform_nth_right (inlineSingle_Meth f)) meths xs)))).
 Proof.
   induction xs; auto.
   simpl.
   intros; specialize (IHxs H).
   destruct (lt_dec a (length meths)).
   - pose proof H0 as H0'.
-    specialize (H0 (fun _ => unit)).
+    specialize (H0).
     inv H0; simpl in *.
     destruct HWfBaseModule as [? [? [NoDupMeths [NoDupRegisters NoDupRle]]]].
     simpl in *.
@@ -3021,15 +3021,15 @@ Qed.
 
 Lemma WfMod_inline_all_Rule regs rules meths f xs:
   In f meths ->
-  (forall ty, WfMod ty (Base (BaseMod regs rules meths))) ->
-  (forall ty, WfMod ty (Base (BaseMod regs (fold_right (transform_nth_right (inlineSingle_Rule f)) rules xs) meths))).
+  (WfMod (Base (BaseMod regs rules meths))) ->
+  (WfMod (Base (BaseMod regs (fold_right (transform_nth_right (inlineSingle_Rule f)) rules xs) meths))).
 Proof.
   induction xs; auto.
   simpl.
   intros; specialize (IHxs H).
   destruct (lt_dec a (length rules)).
   - pose proof H0 as H0'.
-    specialize (H0 (fun _ => unit)).
+    specialize (H0).
     inv H0; simpl in *.
     destruct HWfBaseModule as [? [? [NoDupMeths [NoDupRegisters NoDupRle]]]].
     simpl in *.
@@ -3037,7 +3037,7 @@ Proof.
     rewrite <- (fold_right_len xs (inlineSingle_Rule f) rules) in l.
     specialize (inlineSingle_Rule_transform_nth f _ NoDupRle l) as TMP; dest.
     rewrite H3.
-    specialize (WfMod_Rule_inlined _ (fst x) (IHxs H0' ty) H) as P1.
+    specialize (WfMod_Rule_inlined _ (fst x) (IHxs H0') H) as P1.
     unfold inlineSingle_Rule_BaseModule in P1; simpl in *; assumption.
   - apply Nat.nlt_ge in n.
     rewrite <- (fold_right_len xs (inlineSingle_Rule f) rules) in n.
@@ -3045,14 +3045,14 @@ Proof.
 Qed.
 
 Theorem inline_meth_transform f regs rules meths:
-  (forall ty, WfMod ty (Base (BaseMod regs rules meths))) ->
+  (WfMod (Base (BaseMod regs rules meths))) ->
   In f meths ->
   forall i,
     TraceInclusion (Base (BaseMod regs rules meths)) (Base (BaseMod regs rules (transform_nth_right (inlineSingle_Meth f) i meths))).
 Proof.
   intros; destruct (lt_dec i (length meths)).
   - pose proof H as H'.
-    specialize (H (fun _ => unit)).
+    specialize (H).
     inv H; simpl in *.
     destruct HWfBaseModule as [? [? [NoDupMeths [NoDupRegisters NoDupRle]]]].
     simpl in *.
@@ -3067,14 +3067,14 @@ Proof.
 Qed.
 
 Theorem inline_rule_transform f regs rules meths:
-  (forall ty, WfMod ty (Base (BaseMod regs rules meths))) ->
+  (WfMod (Base (BaseMod regs rules meths))) ->
   In f meths ->
   forall i,
     TraceInclusion (Base (BaseMod regs rules meths)) (Base (BaseMod regs (transform_nth_right (inlineSingle_Rule f) i rules) meths)).
 Proof.
   intros; destruct (lt_dec i (length rules)).
   - pose proof H as H'.
-    specialize (H (fun _ => unit)).
+    specialize (H).
     inv H; simpl in *.
     destruct HWfBaseModule as [? [? [NoDupMeths [NoDupRegisters NoDupRle]]]].
     simpl in *.
@@ -3091,7 +3091,7 @@ Qed.
 Section inlineSingle_nth.
   Variable (f : DefMethT).
   Variable (regs: list RegInitT) (rules: list RuleT) (meths: list DefMethT).
-  Variable (Wf : forall ty, WfMod ty (Base (BaseMod regs rules meths))).
+  Variable (Wf : WfMod (Base (BaseMod regs rules meths))).
 
   Theorem inline_meth_fold_right xs:
     In f meths ->
@@ -3122,7 +3122,7 @@ Section inlineSingle_nth.
 End inlineSingle_nth.
 
 Theorem TraceInclusion_inline_BaseModule_rules regs rules meths f:
-  (forall ty, WfMod ty (Base (BaseMod regs rules meths))) ->
+  (WfMod (Base (BaseMod regs rules meths))) ->
   In f meths ->
   TraceInclusion (Base (BaseMod regs rules meths)) (Base (BaseMod regs (map (inlineSingle_Rule f) rules) meths)).
 Proof.
@@ -3135,7 +3135,7 @@ Proof.
 Qed.
 
 Theorem TraceInclusion_inline_BaseModule_meths regs rules meths f:
-  (forall ty, WfMod ty (Base (BaseMod regs rules meths))) ->
+  (WfMod (Base (BaseMod regs rules meths))) ->
   In f meths ->
   TraceInclusion (Base (BaseMod regs rules meths)) (Base (BaseMod regs rules (map (inlineSingle_Meth f) meths))).
 Proof.
@@ -3149,7 +3149,7 @@ Qed.
 
 
 Theorem TraceInclusion_inline_BaseModule_all regs rules meths f:
-  (forall ty, WfMod ty (Base (BaseMod regs rules meths))) ->
+  (WfMod (Base (BaseMod regs rules meths))) ->
   In f meths ->
   TraceInclusion (Base (BaseMod regs rules meths)) (Base (inlineSingle_BaseModule f regs rules meths)).
 Proof.
@@ -3166,9 +3166,9 @@ Qed.
 
 Section inline_all_all.
   Theorem TraceInclusion_inlineSingle_pos_Rules regs rules meths:
-    (forall ty, WfMod ty (Base (BaseMod regs rules meths))) ->
+    (WfMod (Base (BaseMod regs rules meths))) ->
     forall n,
-      (forall ty, WfMod ty (Base (BaseMod regs (inlineSingle_Rules_pos meths n rules) meths))) /\
+      (WfMod (Base (BaseMod regs (inlineSingle_Rules_pos meths n rules) meths))) /\
       TraceInclusion (Base (BaseMod regs rules meths)) (Base (BaseMod regs (inlineSingle_Rules_pos meths n rules) meths)).
   Proof.
     intros WfH n.
@@ -3184,8 +3184,8 @@ Section inline_all_all.
   Qed.
 
   Theorem TraceInclusion_inlineAll_pos_Rules regs rules meths:
-    (forall ty, WfMod ty (Base (BaseMod regs rules meths))) ->
-    (forall ty, WfMod ty (Base (BaseMod regs (inlineAll_Rules meths rules) meths))) /\
+    (WfMod (Base (BaseMod regs rules meths))) ->
+    (WfMod (Base (BaseMod regs (inlineAll_Rules meths rules) meths))) /\
     TraceInclusion (Base (BaseMod regs rules meths)) (Base (BaseMod regs (inlineAll_Rules meths rules) meths)).
   Proof.
     intros WfH.
@@ -3200,9 +3200,9 @@ Section inline_all_all.
   Qed.
   
   Theorem TraceInclusion_inlineSingle_pos_Meths regs rules meths:
-    (forall ty, WfMod ty (Base (BaseMod regs rules meths))) ->
+    (WfMod (Base (BaseMod regs rules meths))) ->
     forall n,
-      (forall ty, WfMod ty (Base (BaseMod regs rules (inlineSingle_Meths_pos meths n)))) /\
+      (WfMod (Base (BaseMod regs rules (inlineSingle_Meths_pos meths n)))) /\
       TraceInclusion (Base (BaseMod regs rules meths)) (Base (BaseMod regs rules (inlineSingle_Meths_pos meths n))).
   Proof.
     intros WfH n.
@@ -3218,8 +3218,8 @@ Section inline_all_all.
   Qed.
 
   Theorem TraceInclusion_inlineAll_pos_Meths regs rules meths:
-    (forall ty, WfMod ty (Base (BaseMod regs rules meths))) ->
-    (forall ty, WfMod ty (Base (BaseMod regs rules (inlineAll_Meths meths)))) /\
+    (WfMod (Base (BaseMod regs rules meths))) ->
+    (WfMod (Base (BaseMod regs rules (inlineAll_Meths meths)))) /\
     TraceInclusion (Base (BaseMod regs rules meths)) (Base (BaseMod regs rules (inlineAll_Meths meths))).
   Proof.
     intros WfH.
@@ -3234,8 +3234,8 @@ Section inline_all_all.
   Qed.
 
   Theorem TraceInclusion_inlineAll_pos regs rules meths:
-    (forall ty, WfMod ty (Base (BaseMod regs rules meths))) ->
-    (forall ty, WfMod ty (Base (inlineAll_All regs rules meths))) /\
+    (WfMod (Base (BaseMod regs rules meths))) ->
+    (WfMod (Base (inlineAll_All regs rules meths))) /\
     TraceInclusion (Base (BaseMod regs rules meths)) (Base (inlineAll_All regs rules meths)).
   Proof.
     unfold inlineAll_All in *.
@@ -3300,25 +3300,22 @@ Section flatten_and_inline_all.
     unfold inlineAll_Meths; rewrite <-SameKeys_inlineSome_Meths; reflexivity.
   Qed.
   
-  Lemma WfCreateHide_Mod (m : WfModule) ty :
-    WfMod ty (flatten_inline_everything m).
+  Lemma WfCreateHide_Mod (m : ModWf) :
+    WfMod (flatten_inline_everything m).
   Proof.
     unfold flatten_inline_everything, inlineAll_All_module.
-    pose proof (fun ty => flatten_WfMod (Wf_cond m ty)) as HWfm'.
-    pose proof (HWfm' ty) as HWfm.
+    pose proof (flatten_WfMod (Wf_cond m)) as HWfm'.
+    pose proof (HWfm') as HWfm.
     unfold flatten, getFlat in *.
     setoid_rewrite WfMod_createHide in HWfm'; dest.
     rewrite WfMod_createHide in *; dest.
     split; simpl in *.
-    - repeat intro; specialize (H _ H1); rewrite <-SameKeys_inlineAll_Meths; assumption.
-    - match type of HWfm' with
-      | forall ty, _ /\ ?P => assert (Hsth: forall ty, P) by (intros ty0; specialize (HWfm' ty0); tauto)
-      end.
-      apply TraceInclusion_inlineAll_pos in Hsth; dest.
+    - repeat intro; specialize (H _ H3); rewrite <-SameKeys_inlineAll_Meths; assumption.
+    - apply TraceInclusion_inlineAll_pos in H2; dest.
       unfold inlineAll_All in *; auto.
   Qed.
 
-  Definition inlined_WfModule (m : WfModule) : WfModule :=
+  Definition inlined_ModWf (m : ModWf) : ModWf :=
     (mkWfMod (WfCreateHide_Mod m)).
   
   Lemma TraceHide_Trace m o s ls:
@@ -3480,8 +3477,8 @@ Section flatten_and_inline_all.
   Qed.
 
   Lemma WfMod_WfBase_getFlat m:
-    (forall ty, WfMod ty m) ->
-    (forall ty, WfMod ty (Base (getFlat m))).
+    (WfMod m) ->
+    (WfMod (Base (getFlat m))).
   Proof.
     intro.
     induction m; simpl in *.
@@ -3490,38 +3487,36 @@ Section flatten_and_inline_all.
     - intros.
       unfold getFlat in *; simpl in *; apply IHm.
       intros.
-      specialize (H ty0).
+      specialize (H).
       inv H; auto.
     - intros.
-      assert (HWf1: forall ty, WfMod ty m1) by (intros ty0;
-                                                specialize (H ty0);
-                                                inv H; auto).
-      assert (HWf2: forall ty, WfMod ty m2) by (intros ty0;
-                                                specialize (H ty0);
-                                                inv H; auto).
-      assert (WfConcat1: forall ty, WfConcat ty m1 m2) by
-          (intros ty0; specialize (H ty0); inv H; auto).
-      assert (WfConcat2: forall ty, WfConcat ty m2 m1) by
-          (intros ty0; specialize (H ty0); inv H; auto).
-      specialize (H ty).
+      assert (HWf1: WfMod m1) by (specialize (H);
+                                  inv H; auto).
+      assert (HWf2: WfMod m2) by (specialize (H);
+                                  inv H; auto).
+      assert (WfConcat1: WfConcat m1 m2) by
+          (specialize (H); inv H; auto).
+      assert (WfConcat2: WfConcat m2 m1) by
+          (specialize (H); inv H; auto).
+      specialize (H).
       inv H.
       specialize (IHm1 HWf1); specialize (IHm2 HWf2).
       constructor 1;
         ((apply WfMod_WfBaseMod_flat; constructor 3; auto)
-         || (specialize (IHm1 ty);
-             specialize (IHm2 ty);
+         || (specialize (IHm1);
+             specialize (IHm2);
              inv IHm1; inv IHm2;
              simpl in *; apply NoDupKey_Expand; auto)).
   Qed.
   
-  Theorem TraceInclusion_flatten_inline_everything_r (m : WfModule) :
-    TraceInclusion m (inlined_WfModule m).
+  Theorem TraceInclusion_flatten_inline_everything_r (m : ModWf) :
+    TraceInclusion m (inlined_ModWf m).
   Proof.
-    specialize (Wf_cond (inlined_WfModule m)) as Wf1.
+    specialize (Wf_cond (inlined_ModWf m)) as Wf1.
     simpl.
     specialize (TraceInclusion_flatten_r m) as P1.
     unfold flatten, getFlat in *.
-    assert (forall ty, WfMod ty (Base (getFlat m))). {
+    assert (WfMod (Base (getFlat m))). {
       intros.
       apply (WfMod_WfBase_getFlat (Wf_cond m)).
     }
