PProperties.v
@@ -1028,7 +1028,7 @@ Proof.
 Qed.
 
 Lemma PTrace_Trace m o ls:
-  (forall ty, WfMod ty m) ->
+  (WfMod m) ->
   PTrace m o ls ->
   (exists o' ls',
       o' [=] o /\
@@ -1091,8 +1091,8 @@ Proof.
 Qed.
 
 Theorem PTraceInclusion_TraceInclusion m1 m2 :
-  (forall ty, WfMod ty m1) ->
-  (forall ty, WfMod ty m2) ->
+  (WfMod m1) ->
+  (WfMod m2) ->
   PTraceInclusion m1 m2 -> TraceInclusion m1 m2.
 Proof.
   intros.
@@ -1543,12 +1543,12 @@ Proof.
 Qed.
 
 Lemma PStep_substitute' m o l:
-  PStep m o l -> forall (HWfMod: forall ty, WfMod ty m), PStepSubstitute m o l.
+  PStep m o l -> forall (HWfMod: WfMod m), PStepSubstitute m o l.
 Proof.
   intros.
   apply PStep_Step in H; dest.
-  specialize (HWfMod type).
-  apply (@Step_substitute' type) in H2; auto.
+  specialize (HWfMod).
+  apply (@Step_substitute') in H2; auto.
   unfold StepSubstitute in H2; dest.
   unfold PStepSubstitute; repeat split.
   - rewrite H, H1; apply Substeps_PSubsteps; auto.
@@ -1557,7 +1557,7 @@ Proof.
     apply H4; auto.
 Qed.
 
-Lemma PStepSubstitute_flatten m o l (HWfMod: forall ty, WfMod ty m):
+Lemma PStepSubstitute_flatten m o l (HWfMod: WfMod m):
   PStep (flatten m) o l <-> PStepSubstitute m o l.
 Proof.
   unfold flatten, getFlat, PStepSubstitute.
@@ -1582,7 +1582,7 @@ Proof.
       auto.
 Qed.
 
-Lemma PStep_substitute m o l (HWfMod: forall ty, WfMod ty m):
+Lemma PStep_substitute m o l (HWfMod: WfMod m):
   PStep m o l -> PStep (flatten m) o l.
 Proof.
   intros Stp.
@@ -1711,8 +1711,8 @@ Section SplitSubsteps.
   Variable DisjRules: DisjKey (getRules m1) (getRules m2).
   Variable DisjMeths: DisjKey (getMethods m1) (getMethods m2).
 
-  Variable WfMod1: forall ty, WfBaseModule ty m1.
-  Variable WfMod2: forall ty, WfBaseModule ty m2.
+  Variable WfMod1: WfBaseModule m1.
+  Variable WfMod2: WfBaseModule m2.
   
   Lemma pfilter_perm o l :
     PSubsteps (concatFlat m1 m2) o l ->
@@ -1902,7 +1902,7 @@ Lemma flatten_PSubsteps m o l:
   - econstructor 3; eauto.
 Qed.
 
-Lemma substitute_PStep' m (HWfMod: forall ty, WfMod ty m):
+Lemma substitute_PStep' m (HWfMod: WfMod m):
   forall o l,
     PStepSubstitute m o l ->
     PStep m o l.
@@ -1920,7 +1920,7 @@ Proof.
     apply Step_PStep; auto.
 Qed.
 
-Lemma substitute_PStep m o l (HWfMod: forall ty, WfMod ty m):
+Lemma substitute_PStep m o l (HWfMod: WfMod m):
   PStep (flatten m) o l ->
   PStep m o l.
 Proof.
@@ -1930,7 +1930,7 @@ Qed.
 
 Section PTraceSubstitute.
   Variable m: Mod.
-  Variable WfMod_m: forall ty, WfMod ty m.
+  Variable WfMod_m: WfMod m.
 
   Lemma PTrace_flatten_same1: forall o l,  PTrace m o l -> PTrace (flatten m) o l.
   Proof.
@@ -1973,37 +1973,37 @@ Section PTraceSubstitute.
 End PTraceSubstitute.
 
 
-Section WfModule_rewrite.
+Section ModWf_rewrite.
 
-  Inductive WfModule_perm : WfModule ->WfModule -> Prop :=
-  |Wf_perm_equiv (m m': WfModule) (HAllRegsPerm : getAllRegisters m [=] getAllRegisters m')
+  Inductive ModWf_perm : ModWf ->ModWf -> Prop :=
+  |Wf_perm_equiv (m m': ModWf) (HAllRegsPerm : getAllRegisters m [=] getAllRegisters m')
               (HAllMethsPerm : getAllMethods m [=] getAllMethods m')
               (HAllRulesPerm : getAllRules m [=] getAllRules m')
               (HHiddenPerm : getHidden m [=] getHidden m') :
-     WfModule_perm m m'.
+     ModWf_perm m m'.
 
-  Lemma WfModule_perm_refl m :
-    WfModule_perm m m.
+  Lemma ModWf_perm_refl m :
+    ModWf_perm m m.
   Proof.
     constructor; auto.
   Qed.
 
-  Lemma WfModule_perm_sym m m':
-    WfModule_perm m m' -> WfModule_perm m' m.
+  Lemma ModWf_perm_sym m m':
+    ModWf_perm m m' -> ModWf_perm m' m.
   Proof.
     constructor; inv H; eauto using Permutation_sym.
   Qed.
 
-  Lemma WfModule_perm_trans m m' m'' :
-    WfModule_perm m m' -> WfModule_perm m' m'' -> WfModule_perm m m''.
+  Lemma ModWf_perm_trans m m' m'' :
+    ModWf_perm m m' -> ModWf_perm m' m'' -> ModWf_perm m m''.
   Proof.
     constructor; inv H; inv H0; eauto using Permutation_trans.
   Qed.
 
-  Global Instance WfModule_perm_Equivalence : Equivalence (@WfModule_perm) | 10 := {
-     Equivalence_Reflexive := @WfModule_perm_refl;
-     Equivalence_Symmetric := @WfModule_perm_sym;             
-     Equivalence_Transitive:= @WfModule_perm_trans}.
+  Global Instance ModWf_perm_Equivalence : Equivalence (@ModWf_perm) | 10 := {
+     Equivalence_Reflexive := @ModWf_perm_refl;
+     Equivalence_Symmetric := @ModWf_perm_sym;             
+     Equivalence_Transitive:= @ModWf_perm_trans}.
 
   
   Lemma PStep_rewrite_base m1' m2' o l hl:
@@ -2043,8 +2043,8 @@ Proof.
     econstructor 2;[econstructor 2|]; auto.
 Qed.
   
-  Lemma PStep_WfModule_rewrite m1 m2 o l :
-    WfModule_perm m1 m2 ->
+  Lemma PStep_ModWf_rewrite m1 m2 o l :
+    ModWf_perm m1 m2 ->
     PStep m1 o l ->
     PStep m2 o l.
   Proof.
@@ -2085,8 +2085,8 @@ Qed.
       exists x0; split; eauto using Permutation_trans.
   Qed.
   
-  Lemma PTrace_WfModule_rewrite m1 m2 o ls:
-    WfModule_perm m1 m2 ->
+  Lemma PTrace_ModWf_rewrite m1 m2 o ls:
+    ModWf_perm m1 m2 ->
     PTrace m1 o ls ->
     PTrace m2 o ls.
   Proof.
@@ -2095,7 +2095,7 @@ Qed.
       econstructor 1 with (o'':=x);eauto.
       rewrite <- H; assumption.
     - econstructor 2; eauto.
-      eapply (PStep_WfModule_rewrite) in HPStep; eauto.
+      eapply (PStep_ModWf_rewrite) in HPStep; eauto.
       econstructor; eauto.
   Qed.
 
@@ -2118,41 +2118,41 @@ Qed.
 
   Lemma PTrace_rewrite m1 m2 o1 o2 ls:
     o1 [=] o2 ->
-    WfModule_perm m1 m2 ->
+    ModWf_perm m1 m2 ->
     PTrace m1 o1 ls ->
     PTrace m2 o2 ls.
   Proof.
-    intros; eauto using PTrace_WfModule_rewrite, PTrace_RegsT_rewrite.
+    intros; eauto using PTrace_ModWf_rewrite, PTrace_RegsT_rewrite.
   Qed.
 
-  Global Instance PStep_WfModule_rewrite' :
-    Proper (@WfModule_perm ==> Logic.eq ==> Logic.eq ==> iff) (@PStep) |10.
+  Global Instance PStep_ModWf_rewrite' :
+    Proper (@ModWf_perm ==> Logic.eq ==> Logic.eq ==> iff) (@PStep) |10.
   Proof.
-    repeat red; split; intros; subst; eauto using WfModule_perm_sym,PStep_WfModule_rewrite.
+    repeat red; split; intros; subst; eauto using ModWf_perm_sym,PStep_ModWf_rewrite.
   Qed.
 
   Global Instance Trace_rewrite' :
-    Proper (@WfModule_perm ==> @Permutation (string * {x : FullKind & fullType type x}) ==> Logic.eq ==> iff) (@PTrace) | 10.
+    Proper (@ModWf_perm ==> @Permutation (string * {x : FullKind & fullType type x}) ==> Logic.eq ==> iff) (@PTrace) | 10.
   Proof.
-    repeat red; split; intros; subst; eauto using WfModule_perm_sym, Permutation_sym, PTrace_rewrite.
+    repeat red; split; intros; subst; eauto using ModWf_perm_sym, Permutation_sym, PTrace_rewrite.
   Qed.
-End WfModule_rewrite.
+End ModWf_rewrite.
 
-Lemma WfNilMod ty :
-  WfMod ty (Base (BaseMod nil nil nil)).
+Lemma WfNilMod:
+  WfMod (Base (BaseMod nil nil nil)).
 Proof.
   constructor; simpl; constructor; repeat split; intros; try contradiction; simpl; constructor.
 Qed.
 
-Lemma WfConcatActionTNil ty (k : Kind) (a : ActionT ty k):
+Lemma WfConcatActionTNil (k : Kind) (a : ActionT type k):
   WfConcatActionT a (Base (BaseMod nil nil nil)).
 Proof.
   induction a; econstructor; eauto.
 Qed.
 
-Lemma WfConcatNil ty m:
-  WfMod ty m ->
-  WfMod ty (ConcatMod m (Base (BaseMod nil nil nil))).
+Lemma WfConcatNil m:
+  WfMod m ->
+  WfMod (ConcatMod m (Base (BaseMod nil nil nil))).
 Proof.
   constructor; unfold DisjKey; simpl; intros; auto.
   - apply WfNilMod.
@@ -2160,16 +2160,16 @@ Proof.
   - split; intros; contradiction.
 Qed.
 
-Lemma WfNilConcat ty m:
-  WfMod ty (ConcatMod m (Base (BaseMod nil nil nil))) ->
-  WfMod ty m.
+Lemma WfNilConcat m:
+  WfMod (ConcatMod m (Base (BaseMod nil nil nil))) ->
+  WfMod m.
 Proof.
   intros; inv H; assumption.
 Qed.
 
-Lemma WfConcatComm ty m1 m2 :
-  WfMod ty (ConcatMod m1 m2) ->
-  WfMod ty (ConcatMod m2 m1).
+Lemma WfConcatComm m1 m2 :
+  WfMod (ConcatMod m1 m2) ->
+  WfMod (ConcatMod m2 m1).
 Proof.
   intros; inv H.
   econstructor; eauto using DisjKey_Commutative.
@@ -2185,7 +2185,7 @@ Proof.
     intro; destruct H1; auto.
 Qed.
 
-Lemma WfConcatSplits ty m1 m2 (k : Kind) (a : ActionT ty k):
+Lemma WfConcatSplits m1 m2 (k : Kind) (a : ActionT type k):
     WfConcatActionT a (ConcatMod m1 m2) ->
     WfConcatActionT a m1 /\
     WfConcatActionT a m2.
@@ -2206,7 +2206,7 @@ Proof.
   - intros; split; econstructor 10.
 Qed.
 
-Lemma WfConcatMerge ty m1 m2 (k : Kind) (a : ActionT ty k) :
+Lemma WfConcatMerge m1 m2 (k : Kind) (a : ActionT type k) :
   WfConcatActionT a m1 ->
   WfConcatActionT a m2 ->
   WfConcatActionT a (ConcatMod m1 m2).
@@ -2226,9 +2226,9 @@ Proof.
 Qed.
     
 
-Lemma WfConcatAssoc1 ty m1 m2 m3 :
-  WfMod ty (ConcatMod m1 (ConcatMod m2 m3)) ->
-  WfMod ty (ConcatMod (ConcatMod m1 m2) m3).
+Lemma WfConcatAssoc1 m1 m2 m3 :
+  WfMod (ConcatMod m1 (ConcatMod m2 m3)) ->
+  WfMod (ConcatMod (ConcatMod m1 m2) m3).
 Proof.
   intros; inv H; inv HWf2; inv WfConcat1; inv WfConcat2.
   econstructor; simpl in *; eauto.
@@ -2272,9 +2272,9 @@ Proof.
 Qed.
 
 
-Lemma WfConcatAssoc2 ty m1 m2 m3 :
-  WfMod ty (ConcatMod (ConcatMod m1 m2) m3) ->
-  WfMod ty (ConcatMod m1 (ConcatMod m2 m3)).
+Lemma WfConcatAssoc2 m1 m2 m3 :
+  WfMod (ConcatMod (ConcatMod m1 m2) m3) ->
+  WfMod (ConcatMod m1 (ConcatMod m2 m3)).
 Proof.
   intros.
   inv H; inv HWf1; inv WfConcat1; inv WfConcat2.
@@ -2307,7 +2307,7 @@ Proof.
       eauto; eapply (WfConcatSplits (m1 :=m1) (m2 := m2)); eauto.
 Qed.
 
-Lemma WfMod_createHideMod ty l : forall m, WfMod ty (createHideMod m l) <-> (SubList l (map fst (getAllMethods m)) /\ WfMod ty m).
+Lemma WfMod_createHideMod l : forall m, WfMod (createHideMod m l) <-> (SubList l (map fst (getAllMethods m)) /\ WfMod m).
 Proof.
   split.
   - induction l; simpl; intros; split; auto.
@@ -2407,7 +2407,7 @@ Proof.
   repeat red; intros; split; intros; eauto using DisjKey_perm_rewrite, Permutation_sym.
 Qed.
 
-Lemma WfActionTConcatAssoc1 ty m1 m2 m3 (k : Kind) (a : ActionT ty k) :
+Lemma WfActionTConcatAssoc1 m1 m2 m3 (k : Kind) (a : ActionT type k) :
   WfConcatActionT a (ConcatMod (ConcatMod m1 m2) m3) ->
   WfConcatActionT a (ConcatMod m1 (ConcatMod m2 m3)).
 Proof.
@@ -2417,7 +2417,7 @@ Proof.
 Qed.
 
 
-Lemma WfActionTConcatAssoc2 ty m1 m2 m3 (k : Kind) (a : ActionT ty k) :
+Lemma WfActionTConcatAssoc2 m1 m2 m3 (k : Kind) (a : ActionT type k) :
   WfConcatActionT a (ConcatMod m1 (ConcatMod m2 m3)) ->
   WfConcatActionT a (ConcatMod (ConcatMod m1 m2) m3).
 Proof.
@@ -2426,7 +2426,7 @@ Proof.
     rewrite <- app_assoc; assumption.
 Qed.
 
-Lemma WfConcatBaseFiles ty l1 l2 (k : Kind) (a : ActionT ty k):
+Lemma WfConcatBaseFiles l1 l2 (k : Kind) (a : ActionT type k):
   WfConcatActionT a (ConcatMod (mergeSeparatedBaseFile l1) (mergeSeparatedBaseFile l2)) ->
   WfConcatActionT a (mergeSeparatedBaseFile (l1 ++ l2)).
 Proof.
@@ -2440,7 +2440,7 @@ Proof.
     apply WfConcatMerge; eauto.
 Qed.
 
-Lemma WfConcatBaseModules ty l1 l2 (k : Kind) (a : ActionT ty k):
+Lemma WfConcatBaseModules l1 l2 (k : Kind) (a : ActionT type k):
   WfConcatActionT a (ConcatMod (mergeSeparatedBaseMod l1) (mergeSeparatedBaseMod l2)) ->
   WfConcatActionT a (mergeSeparatedBaseMod (l1 ++ l2)).
 Proof.
@@ -2454,11 +2454,11 @@ Proof.
     apply WfConcatMerge; eauto.
 Qed.
 
-Lemma WfAppBaseFiles ty l1 l2:
-  WfMod ty (mergeSeparatedBaseFile l1) ->
-  WfMod ty (mergeSeparatedBaseFile l2) ->
-  WfMod ty (ConcatMod (mergeSeparatedBaseFile l1) (mergeSeparatedBaseFile l2)) ->
-  WfMod ty (mergeSeparatedBaseFile (l1 ++ l2)).
+Lemma WfAppBaseFiles l1 l2:
+  WfMod (mergeSeparatedBaseFile l1) ->
+  WfMod (mergeSeparatedBaseFile l2) ->
+  WfMod (ConcatMod (mergeSeparatedBaseFile l1) (mergeSeparatedBaseFile l2)) ->
+  WfMod (mergeSeparatedBaseFile (l1 ++ l2)).
 Proof.
   induction l1; intros; simpl in *; auto.
   apply WfConcatAssoc2 in H1.
@@ -2479,11 +2479,11 @@ Proof.
     specialize (H3 _ H1 v); assumption.
 Qed.
 
-Lemma WfAppBaseMods ty l1 l2:
-  WfMod ty (mergeSeparatedBaseMod l1) ->
-  WfMod ty (mergeSeparatedBaseMod l2) ->
-  WfMod ty (ConcatMod (mergeSeparatedBaseMod l1) (mergeSeparatedBaseMod l2)) ->
-  WfMod ty (mergeSeparatedBaseMod (l1 ++ l2)).
+Lemma WfAppBaseMods l1 l2:
+  WfMod (mergeSeparatedBaseMod l1) ->
+  WfMod (mergeSeparatedBaseMod l2) ->
+  WfMod (ConcatMod (mergeSeparatedBaseMod l1) (mergeSeparatedBaseMod l2)) ->
+  WfMod (mergeSeparatedBaseMod (l1 ++ l2)).
 Proof.
   induction l1; intros; simpl in *; auto.
   apply WfConcatAssoc2 in H1.
@@ -2509,8 +2509,8 @@ Proof.
 Qed.
 
 
-Lemma Base_File_Disjoint_Registers ty m :
-  WfMod ty m ->
+Lemma Base_File_Disjoint_Registers m :
+  WfMod m ->
   DisjKey (getAllRegisters (mergeSeparatedBaseFile (fst (separateBaseMod m)))) (getAllRegisters (mergeSeparatedBaseMod (snd (separateBaseMod m)))).
 Proof.
   intros; induction m; inv H.
@@ -2542,23 +2542,23 @@ Proof.
       * right; split; auto.
 Qed.
 
-Lemma WfActionBreakDownFile ty m (k : Kind) (a : ActionT ty k): 
+Lemma WfActionBreakDownFile m (k : Kind) (a : ActionT type k): 
   WfConcatActionT a m -> WfConcatActionT a (mergeSeparatedBaseFile (fst (snd (separateMod m)))).
 Proof.
   induction a; simpl; intros; econstructor; intros; try inv H0; try inv H; EqDep_subst; eauto.
   - rewrite mergeSeparatedBaseFile_noHides; intro; contradiction.
 Qed.
 
-Lemma WfActionBreakDownMod ty m (k : Kind) (a : ActionT ty k): 
+Lemma WfActionBreakDownMod m (k : Kind) (a : ActionT type k): 
   WfConcatActionT a m -> WfConcatActionT a (mergeSeparatedBaseMod (snd (snd (separateMod m)))).
 Proof.
   induction a; simpl; intros; econstructor; intros; try inv H0; try inv H; EqDep_subst; eauto.
   - rewrite mergeSeparatedBaseMod_noHides; intro; contradiction.
 Qed.
 
-Lemma WfModBreakDownFile ty m :
-  WfMod ty m ->
-  WfMod ty (mergeSeparatedBaseFile (fst (snd (separateMod m)))).
+Lemma WfModBreakDownFile m :
+  WfMod m ->
+  WfMod (mergeSeparatedBaseFile (fst (snd (separateMod m)))).
 Proof.
   induction m.
   - destruct m; simpl; intros; eauto using WfConcatNil, WfNilMod.
@@ -2602,9 +2602,9 @@ Proof.
         unfold separateMod in H2; simpl in *; rewrite <- Heqsbm1 in H2; simpl in *; assumption.
 Qed.
 
-Lemma WfModBreakDownMod ty m :
-  WfMod ty m ->
-  WfMod ty (mergeSeparatedBaseMod (snd (snd (separateMod m)))).
+Lemma WfModBreakDownMod m :
+  WfMod m ->
+  WfMod (mergeSeparatedBaseMod (snd (snd (separateMod m)))).
 Proof.
   induction m.
   - destruct m; simpl; intros; eauto using WfConcatNil, WfNilMod.
@@ -2648,21 +2648,21 @@ Proof.
         unfold separateMod in H2; simpl in *; rewrite <- Heqsbm1 in H2; simpl in *; assumption.
 Qed.
 
-Lemma WfConcat_noHide ty m1 m2 :
+Lemma WfConcat_noHide m1 m2 :
   getHidden m2 = nil ->
-  WfConcat ty m1 m2.
+  WfConcat m1 m2.
 Proof.
   intros.
   split; intros.
-  - induction (snd rule ty); econstructor; eauto.
+  - induction (snd rule type); econstructor; eauto.
     rewrite H; intro; contradiction.
-  - induction (projT2 (snd meth) ty v); econstructor; eauto.
+  - induction (projT2 (snd meth) type v); econstructor; eauto.
     rewrite H; intro; contradiction.
 Qed.
 
-Lemma merged_WellFormed ty m:
-  WfMod ty m ->
-  WfMod ty (mergeSeparatedMod (separateMod m)).
+Lemma merged_WellFormed m:
+  WfMod m ->
+  WfMod (mergeSeparatedMod (separateMod m)).
 Proof.
   induction 1.
   - destruct m; simpl in *.
@@ -2729,26 +2729,26 @@ Proof.
 Qed.
 
 Lemma WfMod_getFlat m:
-  (forall ty, WfMod ty m) ->
-  (forall ty, WfMod ty (Base (getFlat m))).
+  (WfMod m) ->
+  (WfMod (Base (getFlat m))).
 Proof.
   intros.
   pose proof (WfNoDups H).
   pose proof (WfMod_WfBaseMod_flat H).
-  specialize (H ty).
+  specialize (H).
   unfold getFlat in *.
-  specialize (H1 ty).
+  specialize (H1).
   constructor; tauto.
 Qed.
 
-Definition WfGetFlatMod (m: WfModule) : WfModule :=
-  (mkWfMod (fun ty => Wf_cond m ty)).
+Definition WfGetFlatMod (m: ModWf) : ModWf :=
+  (mkWfMod (Wf_cond m)).
 
-Definition WfMergedMod (m : WfModule) :  WfModule :=
-  (mkWfMod (fun ty => merged_WellFormed (Wf_cond m ty))).
+Definition WfMergedMod (m : ModWf) :  ModWf :=
+  (mkWfMod (merged_WellFormed (Wf_cond m))).
 
 Lemma merged_perm_equality m :
-  WfModule_perm m (WfMergedMod m).
+  ModWf_perm m (WfMergedMod m).
 Proof.
   constructor; simpl.
   - apply separateBaseMod_flatten.
@@ -2757,28 +2757,28 @@ Proof.
   - apply separateBaseModule_flatten_Hides.
 Qed.
 
-Theorem TraceInclusion_Merge_l (m : WfModule) :
+Theorem TraceInclusion_Merge_l (m : ModWf) :
   TraceInclusion m (mergeSeparatedMod (separateMod m)).
 Proof.
   apply PTraceInclusion_TraceInclusion.
   - apply (Wf_cond m).
   - apply (Wf_cond (WfMergedMod m)).
   - repeat intro.
-    apply (PTrace_WfModule_rewrite (merged_perm_equality m)) in H.
+    apply (PTrace_ModWf_rewrite (merged_perm_equality m)) in H.
     exists ls.
     split.
     + unfold PTraceList; exists o; eauto.
     + apply WeakInclusionsRefl.
 Qed.
 
-Theorem TraceInclusion_Merge_r (m : WfModule) :
+Theorem TraceInclusion_Merge_r (m : ModWf) :
   TraceInclusion (mergeSeparatedMod (separateMod m)) m.
 Proof.
   apply PTraceInclusion_TraceInclusion.
   - apply (Wf_cond (WfMergedMod m)).
   - apply (Wf_cond m).
   - repeat intro.
-    apply (PTrace_WfModule_rewrite (WfModule_perm_sym (merged_perm_equality m))) in H.
+    apply (PTrace_ModWf_rewrite (ModWf_perm_sym (merged_perm_equality m))) in H.
     exists ls.
     split.
     + unfold PTraceList; exists o; eauto.
@@ -2787,7 +2787,7 @@ Qed.
 
 Section Comm.
   Variable m1 m2: Mod.
-  Variable wfMod: forall ty, WfMod ty (ConcatMod m1 m2)%kami.
+  Variable wfMod: WfMod (ConcatMod m1 m2)%kami.
 
   Theorem ConcatMod_comm:
     TraceInclusion (ConcatMod m1 m2)%kami (ConcatMod m2 m1)%kami.
@@ -2796,10 +2796,10 @@ Section Comm.
     - intros; eapply WfConcatComm; eauto.
     - unfold PTraceInclusion, TraceList.
       intros.
-      assert (sth: forall ty, WfMod ty (ConcatMod m2 m1)%kami) by (intros; specialize (wfMod ty); eapply WfConcatComm; eauto).
-      assert (sth2: WfModule_perm (mkWfMod wfMod) (mkWfMod sth)) by
+      assert (sth: WfMod (ConcatMod m2 m1)%kami) by (intros; specialize (wfMod); eapply WfConcatComm; eauto).
+      assert (sth2: ModWf_perm (mkWfMod wfMod) (mkWfMod sth)) by
           (constructor; simpl; auto; apply Permutation_app_comm).
-      pose proof (@PTrace_WfModule_rewrite (mkWfMod wfMod) (mkWfMod sth) o ls sth2 H).
+      pose proof (@PTrace_ModWf_rewrite (mkWfMod wfMod) (mkWfMod sth) o ls sth2 H).
       exists ls.
       split.
       + exists o; auto.
@@ -2809,7 +2809,7 @@ End Comm.
 
 Section Assoc.
   Variable m1 m2 m3: Mod.
-  Variable wfMod: forall ty, WfMod ty (ConcatMod (ConcatMod m1 m2) m3)%kami.
+  Variable wfMod: WfMod (ConcatMod (ConcatMod m1 m2) m3)%kami.
 
   Theorem ConcatModAssoc1:
     TraceInclusion (ConcatMod m1 (ConcatMod m2 m3))%kami (ConcatMod (ConcatMod m1 m2) m3)%kami.
@@ -2818,10 +2818,10 @@ Section Assoc.
     - intros; eapply WfConcatAssoc2; eauto.
     - unfold PTraceInclusion, TraceList.
       intros.
-      assert (sth: forall ty, WfMod ty (ConcatMod m1 (ConcatMod m2 m3))%kami) by (intros; specialize (wfMod ty); eapply WfConcatAssoc2; eauto).
-      assert (sth2: WfModule_perm (mkWfMod sth) (mkWfMod wfMod)) by
+      assert (sth: WfMod (ConcatMod m1 (ConcatMod m2 m3))%kami) by (intros; specialize (wfMod); eapply WfConcatAssoc2; eauto).
+      assert (sth2: ModWf_perm (mkWfMod sth) (mkWfMod wfMod)) by
         (constructor; simpl; rewrite app_assoc; auto).
-      pose proof (@PTrace_WfModule_rewrite (mkWfMod sth) (mkWfMod wfMod) o ls sth2 H).
+      pose proof (@PTrace_ModWf_rewrite (mkWfMod sth) (mkWfMod wfMod) o ls sth2 H).
       exists ls.
       split.
       + exists o; auto.
@@ -2835,10 +2835,10 @@ Section Assoc.
     - intros; eapply WfConcatAssoc2; eauto.
     - unfold PTraceInclusion, TraceList.
       intros.
-      assert (sth: forall ty, WfMod ty (ConcatMod m1 (ConcatMod m2 m3))%kami) by (intros; specialize (wfMod ty); eapply WfConcatAssoc2; eauto).
-      assert (sth2: WfModule_perm (mkWfMod wfMod) (mkWfMod sth)) by
+      assert (sth: WfMod (ConcatMod m1 (ConcatMod m2 m3))%kami) by (intros; specialize (wfMod); eapply WfConcatAssoc2; eauto).
+      assert (sth2: ModWf_perm (mkWfMod wfMod) (mkWfMod sth)) by
         (constructor; simpl; rewrite app_assoc; auto).
-      pose proof (@PTrace_WfModule_rewrite (mkWfMod wfMod) (mkWfMod sth) o ls sth2 H).
+      pose proof (@PTrace_ModWf_rewrite (mkWfMod wfMod) (mkWfMod sth) o ls sth2 H).
       exists ls.
       split.
       + exists o; auto.
